partial/Exception.v
@@ -1,0 +1,213 @@
+(** Calculation of the simple arithmetic language. *)
+
+Require Import List.
+Require Import Tactics.
+Require Import Coq.Program.Equality.
+Module Exception (mem : Memory).
+Import mem.
+
+  
+(** * Syntax *)
+
+Inductive Expr : Set := 
+| Val : nat -> Expr 
+| Add : Expr -> Expr -> Expr
+| Throw : Expr 
+| Catch : Expr -> Expr -> Expr.
+
+(** * Semantics *)
+
+Fixpoint eval (x: Expr) : option nat :=
+  match x with
+    | Val n => Some n
+    | Add x1 x2 => match eval x1 with
+                   | Some m => match eval x2 with
+                               | Some n => Some (m + n)%nat
+                               | None => None
+                               end
+                   | None => None
+                   end
+    | Throw => None
+    | Catch x h => match eval x with
+                   | Some n => Some n
+                   | None => eval h
+                   end 
+  end.
+
+(** * Compiler *)
+
+Inductive Code : Set :=
+| LOAD : nat -> Code -> Code
+| ADD : adr -> Code -> Code
+| STORE : adr -> Code -> Code
+| THROW : Code
+| UNMARK : Code -> Code
+| MARK : adr -> Code -> Code -> Code
+| HALT : Code.
+
+Fixpoint comp' (x : Expr) (r : adr) (c : Code) : Code :=
+  match x with
+  | Val n => LOAD n c
+  | Add e1 e2 => comp' e1 r (STORE r (comp' e2 (next r) (ADD r c)))
+  | Throw => THROW
+  | Catch e1 e2 => MARK r (comp' e2 r c) (comp' e1 (next r) (UNMARK c))
+  end.
+
+Definition comp (x : Expr) : Code := comp' x adr0 HALT.
+
+Definition Han := option adr.
+
+Inductive Elem : Set :=
+| NUM : nat -> Elem
+| HAN : Code -> Han -> Elem.
+
+(** * Virtual Machine *)
+
+Inductive Conf : Type :=
+| conf : Code -> nat -> Han -> Conf
+| fail : nat -> Han -> Conf.
+
+
+Notation "⟨ x , y , z , s ⟩" := (conf x y z, s).
+Notation "⟪ x , y , s ⟫" := (fail x y, s).
+
+Reserved Notation "x ==> y" (at level 80, no associativity).
+Inductive VM : Conf * Mem Elem -> Conf * Mem Elem -> Prop :=
+| vm_load n a c s p : ⟨LOAD n c, a , p, s⟩ ==> ⟨c , n, p, s⟩ 
+| vm_add c s a r n p : s[r]=  NUM n -> ⟨ADD r c, a , p, s⟩ ==> ⟨c , n + a, p, s⟩
+| vm_store c s a r p : ⟨STORE r c, a, p, s⟩ ==> ⟨c , a, p, s[r:=NUM a]⟩
+| vm_throw a s p : ⟨THROW, a, p, s⟩ ==> ⟪a, p, s⟫
+| vm_fail p p' a s c : s[p] = HAN c p' -> ⟪a, Some p, s⟫ ==> ⟨c, a, p', s⟩
+| vm_unmark p p' s a c c' : s[p] = HAN c' p' ->
+                            ⟨UNMARK c, a, Some p, s⟩ ==> ⟨c, a, p', s⟩
+| vm_mark p r s a c c' : ⟨MARK r c' c, a, p, s⟩ ==> ⟨c, a, Some r, s[r:= HAN c' p]⟩
+where "x ==> y" := (VM x y).
+
+
+
+(** * Calculation *)
+
+(** Boilerplate to import calculation tactics *)
+Module Mon := Monotonicity mem.
+Import Mon.
+
+Module VM <: (Machine mem).
+Definition Conf := Conf.
+Definition Rel := VM.
+Definition MemElem := Elem.
+Lemma monotone : monotonicity VM.
+prove_monotonicity. Qed.
+End VM.
+Module VMCalc := Calculation mem VM.
+Import VMCalc.
+
+
+(** Specification of the compiler *)
+
+Theorem spec e r c a p s :
+  freeFrom r s ->
+  ⟨comp' e r c, a, p, s⟩
+    =|>
+    match eval e with
+    | Some n => ⟨c , n, p, s⟩
+    | None => ⟪a, p, s⟫
+    end.
+
+
+(** Setup the induction proof *)
+
+Proof.
+  intros.
+  generalize dependent c.
+  generalize dependent s.
+  generalize dependent r.
+  generalize dependent a.
+  generalize dependent p.
+  induction e;intros.
+
+(** Calculation of the compiler *)
+
+(** - [x = Val n]: *)
+
+  begin
+    match eval (Val n) with
+    | Some n' => ⟨c , n' ,p, s⟩
+    | None => ⟪ a, p, s⟫
+    end.
+  = {auto}
+      ⟨ c, n, p, s⟩.
+  <== {apply vm_load}
+      ⟨ LOAD n c, a, p, s ⟩.
+  [].
+
+(** - [x = Add x1 x2]: *)
+  
+  begin
+    match eval (Add e1 e2) with
+    | Some n => ⟨c , n ,p, s⟩
+    | None => ⟪ a, p, s⟫
+    end.
+  = { auto }
+    match eval e1 with
+    | Some n => match eval e2 with
+                | Some n' => ⟨c , n + n' ,p, s⟩
+                | None => ⟪ a, p, s⟫
+                end
+    | None => ⟪ a, p, s⟫
+    end.
+  ≤ { auto }
+    match eval e1 with
+    | Some n => match eval e2 with
+                | Some n' => ⟨c , n + n' ,p, s[r:=NUM n]⟩
+                | None => ⟪ a, p, s[r:=NUM n]⟫
+                end
+    | None => ⟪ a, p, s⟫
+    end.
+  <== {apply vm_add; eauto using get_set}
+      match eval e1 with
+      | Some n => match eval e2 with
+                  | Some n' => ⟨ADD r c , n' ,p, s[r:=NUM n]⟩
+                  | None => ⟪ a, p, s[r:=NUM n]⟫
+                  end
+      | None => ⟪ a, p, s⟫
+      end.
+  <|= {?}
+      match eval e1 with
+      | Some n => ⟨comp' e2 (next r) (ADD r c) , a ,p, s[r:=NUM n]⟩
+      | None => ⟪ a, p, s⟫
+      end.
+dist; eauto using freeFrom_set,IHe2.
+  
+      ⟨comp' e2 (next r) (ADD r c), eval e1, set r (eval e1) s⟩.
+  <== { apply vm_store}
+    ⟨STORE r (comp' e2 (next r) (ADD r c)), eval e1, s⟩.
+  <|= { apply IHe1;eauto }
+    ⟨comp' e1 r (STORE r (comp' e2 (next r) (ADD r c))), a, s⟩.
+  [].
+Qed.
+
+
+(** * Soundness *)
+  
+(** Since the VM is defined as a small step operational semantics, we *)
+(* have to prove that the VM is deterministic and does not get stuck in *)
+(* order to derive soundness from the above theorem. *)
+
+
+Lemma determ_vm : determ VM.
+  intros C C1 C2 V. induction V; intro V'; inversion V'; subst;eauto.
+  rewrite H in *. inversion H5;subst. auto.
+Qed.
+
+
+Theorem sound x a s C : freeFrom adr0 s -> ⟨comp x, a, s⟩ =>>! C -> exists s', C = ⟨HALT, eval x, s'⟩.
+Proof.
+  intros F M.
+  pose (spec x adr0 HALT a s F). unfold Reach in *. repeat autodestruct.
+  pose (determ_trc determ_vm) as D.
+  unfold determ in D. inversion H0. subst. eexists. eapply D. apply M. split. 
+  apply H. intro Contra. destruct Contra.
+  inversion H1.
+Qed.
+
+End Arith.
